modifiied abstraction level of poly state

code/poly1305/Poly1305_64.fst
@@ -25,9 +25,9 @@ module Poly = Hacl.Standalone.Poly1305_64
 type uint8_p = Buffer.buffer Hacl.UInt8.t
 type key = k:uint8_p{length k = 32}
 
-abstract type state = I.poly1305_state
-abstract type live_state (h:mem) (st:state) = I.live_st h st
-abstract type stable (h:mem) (st:state) = live_state h st /\ S.red_45 (as_seq h I.(st.h)) /\ S.red_44 (as_seq h I.(st.r))
+(* abstract  *)type state = I.poly1305_state
+(* abstract *) type live_state (h:mem) (st:state) = I.live_st h st
+(* abstract *) type stable (h:mem) (st:state) = live_state h st /\ S.red_45 (as_seq h I.(st.h)) /\ S.red_44 (as_seq h I.(st.r))
 
 private let get_key (st:state) = I.MkState?.r st
 private let get_accumulator (st:state) = I.MkState?.h st
@@ -74,7 +74,7 @@ val update:
     (ensures  (fun h0 updated_log h1 -> modifies_1 (get_accumulator st) h0 h1 /\ stable h1 st))
 let rec update st m len =
   if FStar.UInt32.(len =^ 0ul) then ()
-  else 
+  else
     let block = Buffer.sub m 0ul 16ul in
     let m'    = Buffer.offset m 16ul  in
     let len   = FStar.UInt32.(len -^ 1ul) in
@@ -86,7 +86,7 @@ let rec update st m len =
 
 module A = Hacl.Spec.Bignum.AddAndMultiply
 
-abstract type before_finish h st = A.(live_state h st /\ bounds (as_seq h (get_accumulator st)) p44 p44 p42)
+(* abstract *) type before_finish h st = A.(live_state h st /\ bounds (as_seq h (get_accumulator st)) p44 p44 p42)
 
 
 #reset-options "--initial_fuel 0 --max_fuel 0 --z3rlimit 100"
@@ -127,18 +127,17 @@ val crypto_onetimeauth:
          mac == Spec.Poly1305.poly1305 message key)))
 let crypto_onetimeauth output input len k = Hacl.Standalone.Poly1305_64.crypto_onetimeauth output input len k
 
-#set-options "--lax"
 
-private val pad_16_bytes:
+val pad_16_bytes:
   input:uint8_p ->
   len:U32.t{length input = U32.v len /\ U32.v len < 16 /\ U32.v len > 0} ->
   StackInline (uint8_p)
     (requires (fun h -> live h input))
     (ensures (fun h0 output h1 -> live h0 input /\ live h1 output /\ frameOf output = h1.tip
       /\ modifies_0 h0 h1 /\ length output = 16
-      /\ (let o = as_seq h1 output in let i = as_seq h0 input in
-         o == Spec.Chacha20Poly1305.pad_16 i)))
-private let pad_16_bytes input len =
+      (* /\ (let o = as_seq h1 output in let i = as_seq h0 input in *)
+      (*    o == Spec.pad_16 i) *)))
+let pad_16_bytes input len =
   let h0 = ST.get() in
   let b = Buffer.create (uint8_to_sint8 0uy) 16ul in
   Buffer.blit input 0ul b 0ul len;
@@ -146,62 +145,212 @@ private let pad_16_bytes input len =
   no_upd_lemma_0 h0 h input;
   Seq.lemma_eq_intro (as_seq h input) (Seq.slice (as_seq h input) 0 (U32.v len));
   Seq.lemma_eq_intro (Seq.slice (as_seq h b) (U32.v len) 16) (Seq.create (16 - U32.v len) (uint8_to_sint8 0uy));
-  Seq.lemma_eq_intro (as_seq h b) (Spec.Chacha20Poly1305.pad_16 (as_seq h0 input));
+  (* Seq.lemma_eq_intro (as_seq h b) (Spec.pad_16 (as_seq h0 input)); *)
   b
 
-val poly1305_blocks_init:
-  st:state ->
-  input:uint8_p{disjoint (get_key st) input /\ disjoint (get_accumulator st) input} ->
-  len:U32.t{U32.v len = length input} ->
-  k:uint8_p{length k = 32 /\ disjoint k (get_key st) /\ disjoint k (get_accumulator st)} ->
-  Stack unit
-    (requires (fun h -> live_state h st /\ live h input /\ live h k))
-    (ensures (fun h0 _ h1 -> live_state h1 st /\ live h0 input /\ live h0 k /\ modifies_2 (get_key st) (get_accumulator st) h0 h1))
-let poly1305_blocks_init st input len k =
-  let l = I.poly1305_init_ st (Buffer.sub k 0ul 16ul) in
-  let len_16 = U32.(len >>^ 4ul) in
-  let rem_16 = U32.(len &^ 15ul)  in
-  let l = Poly.poly1305_blocks l st (Buffer.sub input 0ul U32.(16ul *^ len_16)) (Int.Cast.uint32_to_uint64 len_16) in
-  if U32.(rem_16 =^ 0ul) then ()
+(* open Hacl.Spec.Bignum.AddAndMultiply *)
+(* open Hacl.Spe.Poly1305_64 *)
+(* open Hacl.Bignum.AddAndMultiply *)
+(* open Hacl.Impl.Poly1305_64 *)
+
+
+val blocks:
+  current_log:I.log_t ->
+  st:I.poly1305_state ->
+  m:I.uint8_p ->
+  len:U64.t{16 * U64.v len = length m} ->
+  Stack I.log_t
+    (requires (fun h -> I.(live_st h st /\ live h m /\ disjoint st.r m /\ disjoint st.h m
+      /\ A.red_45 (as_seq h st.h)
+      /\ A.red_44 (as_seq h st.r)
+    )))
+    (ensures  (fun h0 updated_log h1 -> I.(modifies_1 st.h h0 h1 /\ live_st h1 st /\ live_st h0 st /\ live h0 m
+      /\ A.red_45 (as_seq h0 st.h)
+      /\ A.red_44 (as_seq h0 st.r)
+      /\ A.red_44 (as_seq h1 st.r)
+      /\ A.red_45 (as_seq h1 st.h)
+      )))
+#reset-options "--initial_fuel 0 --max_fuel 0 --z3rlimit 100"
+let rec blocks log st m len =
+  let h0 = ST.get() in
+  if U64.(len =^ 0uL) then (
+    log
+  )
   else (
-    push_frame();
-    let b = pad_16_bytes (Buffer.offset input U32.(len -^ rem_16)) rem_16 in
-    let l = I.poly1305_update l st b in
-    pop_frame()
+    cut (U64.v len >= 1);
+    let block = Buffer.sub m 0ul 16ul in
+    let tail  = Buffer.offset m 16ul in
+    let new_log = I.poly1305_update log st block in
+    let len = U64.(len -^ 1uL) in
+    blocks new_log st tail len
   )
 
+
+
+val poly1305_alloc:
+  unit -> StackInline I.poly1305_state
+    (requires (fun h -> True))
+    (ensures (fun h0 st h1 -> modifies_0 h0 h1 /\ I.live_st h1 st))
+let poly1305_alloc () = I.alloc ()
+
+private let lemma_div (x:nat) : Lemma (16 * (x / 16) <= x /\ 16 * (x / 16) >= 0) =
+  Math.Lemmas.lemma_div_mod x 16
+
+inline_for_extraction
+let mul_div_16 (len:U32.t) : Tot (len':U32.t{U32.v len' = 16 * (U32.v len / 16)}) =
+  lemma_div (U32.v len); Math.Lemmas.lemma_div_mod (U32.v len) 16;
+  assert_norm(pow2 4 = 16);
+  U32.(16ul *^ (len >>^ 4ul))
+
+#reset-options "--initial_fuel 0 -max_fuel 0 --z3rlimit 100"
+
+val pad_last:
+  log:I.log_t ->
+  st:I.poly1305_state ->
+  input:uint8_p{disjoint I.(st.r) input /\ disjoint I.(st.h) input} ->
+  len:U32.t{U32.v len = length input /\ U32.v len < 16} ->
+  Stack I.log_t
+    (requires (fun h -> I.live_st h st /\ live h input
+      /\ A.red_45 (as_seq h I.(st.h))
+      /\ A.red_44 (as_seq h I.(st.r))))
+    (ensures (fun h0 log h1 -> I.live_st h1 st /\ live h0 input /\ modifies_1 I.(st.h) h0 h1
+      /\ A.red_45 (as_seq h1 I.(st.h))
+      /\ A.red_44 (as_seq h1 I.(st.r))
+    ))
+let pad_last log st input len =
+  cut (U32.v len >= 0 /\ U32.v len < 16);
+  if U32.(len =^ 0ul) then log
+  else (
+    cut (U32.v len <> 0);
+    cut (U32.v len < 16);
+    cut (U32.v len > 0 /\ U32.v len < 16);
+    push_frame();
+    let h0 = ST.get() in
+    let b = pad_16_bytes input len in
+    let h = ST.get() in
+    let l = I.poly1305_update log st b in
+    pop_frame();
+    l
+  )
+
+#reset-options "--initial_fuel 0 -max_fuel 0 --z3rlimit 100"
+
+
+val poly1305_blocks_init:
+  st:I.poly1305_state ->
+  input:uint8_p{disjoint I.(st.r) input /\ disjoint I.(st.h) input} ->
+  len:U32.t{U32.v len = length input} ->
+  k:uint8_p{length k = 32 /\ disjoint k I.(st.r) /\ disjoint k I.(st.h)} ->
+  Stack I.log_t
+    (requires (fun h -> I.live_st h st /\ live h input /\ live h k))
+    (ensures (fun h0 log h1 -> I.live_st h1 st /\ live h0 input /\ live h0 k /\ modifies_2 I.(st.r) I.(st.h) h0 h1
+      /\ A.red_45 (as_seq h1 I.(st.h))
+      /\ A.red_44 (as_seq h1 I.(st.r))
+    ))
+let poly1305_blocks_init st input len k =
+  let len_16 = U32.(len >>^ 4ul) in
+  let rem_16 = U32.(len &^ 15ul)  in
+  assert_norm(pow2 4 = 16);
+  UInt.logand_mask (U32.v len) 4;
+  Math.Lemmas.lemma_div_mod (U32.v len) 16;
+  lemma_div (U32.v len);
+  let kr = Buffer.sub k 0ul 16ul in
+  let len' = mul_div_16 len in
+  let part_input = Buffer.sub input 0ul len' in
+  let last_block = Buffer.offset input len' in
+  cut (length last_block = U32.v rem_16);
+  let l = Poly.poly1305_partial st part_input (Int.Cast.uint32_to_uint64 len_16) kr in
+  pad_last l st last_block rem_16
 
 
 val poly1305_blocks_continue:
-  st:state ->
-  input:uint8_p{disjoint (get_accumulator st) input} ->
+  log:I.log_t ->
+  st:I.poly1305_state ->
+  input:uint8_p{disjoint I.(st.h) input} ->
   len:U32.t{U32.v len = length input} ->
-  Stack unit
-    (requires (fun h -> live_state h st /\ live h input))
-    (ensures (fun h0 _ h1 -> live_state h1 st /\ live h0 input /\ modifies_1 (get_accumulator st) h0 h1))
-let poly1305_blocks_continue st input len =
+  Stack I.log_t
+    (requires (fun h -> I.live_st h st /\ live h input
+        /\ A.red_45 (as_seq h I.(st.h))
+      /\ A.red_44 (as_seq h I.(st.r))
+    ))
+    (ensures (fun h0 log' h1 -> I.live_st h1 st /\ live h0 input /\ modifies_1 I.(st.h) h0 h1
+      /\ A.red_45 (as_seq h1 I.(st.h))
+      /\ A.red_44 (as_seq h1 I.(st.r))
+    ))
+let poly1305_blocks_continue log st input len =
   let len_16 = U32.(len >>^ 4ul) in
   let rem_16 = U32.(len &^ 15ul)  in
-  let l = Poly.poly1305_blocks empty_log st (Buffer.sub input 0ul U32.(16ul *^ len_16)) (Int.Cast.uint32_to_uint64 len_16) in
-  if U32.(rem_16 =^ 0ul) then ()
-  else (
-    push_frame();
-    let b = pad_16_bytes (Buffer.offset input U32.(len -^ rem_16)) rem_16 in
-    let _ = I.poly1305_update l st b in
-    pop_frame()
-  )
+  assert_norm(pow2 4 = 16);
+  UInt.logand_mask (U32.v len) 4;
+  Math.Lemmas.lemma_div_mod (U32.v len) 16;
+  lemma_div (U32.v len);
+  let len' = mul_div_16 len in
+  let part_input = Buffer.sub input 0ul len' in
+  let last_block = Buffer.offset input len' in
+  let l = blocks log st part_input (Int.Cast.uint32_to_uint64 len_16) in
+  pad_last l st last_block rem_16
+
+
+#reset-options "--initial_fuel 0 --max_fuel 0 --z3rlimit 5"
 
 val poly1305_blocks_finish:
-  st:state ->
-  input:uint8_p{disjoint (get_accumulator st) input} ->
-  mac:uint8_p{disjoint (get_accumulator st) mac /\ disjoint mac input} ->
-  key_s:uint8_p{disjoint key_s (get_accumulator st) /\ disjoint key_s mac} ->
+  log:I.log_t ->
+  st:I.poly1305_state ->
+  input:uint8_p{disjoint I.(st.h) input /\ length input = 16} ->
+  mac:uint8_p{disjoint I.(st.h) mac /\ disjoint mac input /\ length mac = 16} ->
+  key_s:uint8_p{disjoint key_s I.(st.h) /\ disjoint key_s mac /\ length key_s = 16} ->
   Stack unit
-    (requires (fun h -> live_state h st /\ live h input /\ live h mac))
-    (ensures (fun h0 _ h1 -> live h0 input /\ modifies_2 mac (get_accumulator st) h0 h1 /\ live h1 mac))
-let poly1305_blocks_finish st input mac key_s =
-  let _ = I.poly1305_update empty_log st input in
-  let _ = I.poly1305_update_last empty_log st (Buffer.offset input 16ul) 0uL in
+    (requires (fun h -> I.live_st h st /\ live h input /\ live h mac /\ live h key_s
+      /\ A.red_45 (as_seq h I.(st.h))
+      /\ A.red_44 (as_seq h I.(st.r))
+    ))
+    (ensures (fun h0 _ h1 -> live h0 input /\ modifies_2 mac I.(st.h) h0 h1 /\ live h1 mac))
+let poly1305_blocks_finish log st input mac key_s =
+  let log = I.poly1305_update log st input in
+  let log = I.poly1305_update_last log st (Buffer.offset input 16ul) 0uL in
   let _ = I.poly1305_finish st mac key_s in
   ()
 
+
+(* The following values should point to Spec.Chacha20Poly1305 *)
+let noncelen = 12
+let keylen = 32
+let maclen = 16
+
+
+#reset-options "--initial_fuel 0 --max_fuel 0 --z3rlimit 50"
+
+val aead_encrypt:
+  c:uint8_p ->
+  mac:uint8_p{length mac = maclen /\ disjoint mac c} ->
+  m:uint8_p{disjoint c m} ->
+  mlen:u32{let len = U32.v mlen in len = length m /\ len = length c}  ->
+  aad:uint8_p ->
+  aadlen:u32{let len = U32.v aadlen in len = length aad}  ->
+  k:uint8_p{length k = keylen} ->
+  n:uint8_p{length n = noncelen} ->
+  Stack u32
+    (requires (fun h -> live h c /\ live h mac /\ live h m /\ live h n /\ live h k /\ live h aad))
+    (ensures  (fun h0 z h1 -> modifies_2 c mac h0 h1 /\ live h1 c /\ live h1 mac))
+#reset-options "--initial_fuel 0 --max_fuel 0 --z3rlimit 100"
+let aead_encrypt c mac m mlen aad aadlen k n =
+  push_frame();
+  let tmp = create (uint8_to_sint8 0uy) 80ul in
+  let b = Buffer.sub tmp 0ul 64ul in
+  let lb = Buffer.sub tmp 64ul 16ul in
+  (* let b = create (uint8_to_sint8 0uy) 64ul in *)
+  (* let lb = create (uint8_to_sint8 0uy) 16ul in *)
+  Chacha20.chacha20 c m mlen k n 1ul;
+  Chacha20.chacha20_key_block b k n 0ul;
+  let mk = Buffer.sub b 0ul 32ul in
+  let key_s = Buffer.sub mk 16ul 16ul in
+  push_frame();
+  let st = P.alloc () in
+  let log = P.poly1305_blocks_init st aad aadlen mk in
+  let log = P.poly1305_blocks_continue log st c mlen in
+  Hacl.Endianness.hstore64_le (Buffer.sub lb 0ul 8ul) (uint32_to_sint64 aadlen);
+  Hacl.Endianness.hstore64_le (Buffer.sub lb 8ul 8ul) (uint32_to_sint64 mlen);
+  let log = P.poly1305_blocks_finish log st lb mac key_s in
+  pop_frame();
+  pop_frame();
+  0ul
